Checkpoint progress on file_truncate

src/AsyncFS.v
@@ -13,7 +13,7 @@ Require Import ListPred.
 Require Import SepAuto.
 Require Import Idempotent.
 Require Import Inode.
-Require Import List.
+Require Import List ListUtils.
 Require Import Balloc.
 Require Import Bytes.
 Require Import DirTree.
@@ -30,7 +30,6 @@ Require Import NEList.
 
 Set Implicit Arguments.
 Import ListNotations.
-
 
 
 Module AFS.
@@ -69,10 +68,16 @@ Module AFS.
       mscs <- LOG.commit_ro (FSXPLog fsxp) mscs;
         rx ^(mscs, b).
 
-  Definition truncate T fsxp inum sz mscs rx : prog T :=
-     mscs <- LOG.begin (FSXPLog fsxp) mscs;
-     let^ (mscs, ok) <- BFILE.truncate (FSXPLog fsxp) (FSXPBlockAlloc fsxp) (FSXPInode fsxp) inum sz mscs;
-     rx ^(mscs, ok).
+  Definition file_truncate T fsxp inum sz ms rx : prog T :=
+    ms <- LOG.begin (FSXPLog fsxp) ms;
+    let^ (ms, ok) <- BFILE.truncate (FSXPLog fsxp) (FSXPBlockAlloc fsxp) (FSXPInode fsxp) inum sz ms;
+    If (bool_dec ok false) {
+      ms <- LOG.abort (FSXPLog fsxp) ms;
+      rx ^(ms, false)
+    } else {
+      let^ (ms, ok) <- LOG.commit (FSXPLog fsxp) ms;
+      rx ^(ms, ok)
+    }.
 
   (* update an existing block directly.  XXX dwrite happens to sync metadata. *)
   Definition update_fblock_d T fsxp inum off v ms rx : prog T :=
@@ -85,34 +90,6 @@ Module AFS.
   Definition file_sync T fsxp inum ms rx : prog T :=
     ms <- BFILE.datasync (FSXPLog fsxp) (FSXPInode fsxp) inum ms;
     rx ms.
-
-(*
-
-  Definition write_block T fsxp inum off v newsz mscs rx : prog T :=
-    mscs <- LOG.begin (FSXPLog fsxp) mscs;
-    let^ (mscs, oldattr) <- BFILE.getattrs (FSXPLog fsxp) (FSXPInode fsxp) inum mscs;
-      let^ (mscs, curlen) <- BFILE.getlen (FSXPLog fsxp) (FSXPInode fsxp) inum mscs;
-        mscs <- IfRx irx (lt_dec off curlen) {
-               irx mscs
-             } else {
-      let^ (mscs, ok) <- BFILE.truncate (FSXPLog fsxp) (FSXPBlockAlloc fsxp) (FSXPInode fsxp) inum (off + 1) mscs;
-         If (bool_dec ok true) {
-              irx mscs
-            } else {
-          mscs <- LOG.abort (FSXPLog fsxp) mscs;
-          rx ^(mscs, false)
-        }
-    };
-    mscs <- BFILE.write (FSXPLog fsxp) (FSXPInode fsxp) inum off v mscs;
-    mscs <- IfRx irx (wlt_dec (INODE.ABytes oldattr) newsz) {
-           mscs <- BFILE.updattr (FSXPLog fsxp) (FSXPInode fsxp) inum (INODE.UBytes newsz) mscs;
-           irx mscs
-         } else {
-      irx mscs
-    };
-    let^ (mscs, ok) <- LOG.commit (FSXPLog fsxp) mscs;
-      rx ^(mscs, ok).
-*)
 
   Definition readdir T fsxp dnum mscs rx : prog T :=
     mscs <- LOG.begin (FSXPLog fsxp) mscs;
@@ -195,7 +172,6 @@ Module AFS.
       rx ^(mscs, false)
     }.
 
-
   (* sync directory tree; will flush all outstanding changes to tree (but not dupdates to files) *)
   Definition tree_sync T fsxp mscs rx : prog T :=
     mscs <- GLog.flushall fsxp mscs;
@@ -250,7 +226,6 @@ Module AFS.
     intuition eauto.
   Qed.
 
-
   Ltac recover_ro_ok := intros;
     repeat match goal with
       | [ |- forall_helper _ ] => idtac "forall"; unfold forall_helper; intros; eexists; intros
@@ -261,7 +236,6 @@ Module AFS.
       | [ H: diskIs _ _ |- _ ] => idtac "unfold"; unfold diskIs in *
       | [ |- pimpl (crash_xform _) _ ] => idtac "crash_xform"; progress autorewrite with crash_xform
     end.
-
 
   Hint Extern 0 (okToUnify (LOG.idempred _ _ _) (LOG.idempred _ _ _)) => constructor : okToUnify.
   Hint Extern 0 (okToUnify (LOG.after_crash _ _ _ _) (LOG.after_crash _ _ _ _)) => constructor : okToUnify.
@@ -285,7 +259,6 @@ Module AFS.
 
   (* Specs and proofs *)
 
-
   Theorem file_getattr_ok : forall fsxp inum mscs,
   {< ds pathname Fm Ftop tree f,
   PRE    LOG.rep (FSXPLog fsxp) (SB.rep fsxp) (LOG.NoTxn ds) mscs  *
@@ -308,8 +281,7 @@ Module AFS.
     rewrite LOG.notxn_idempred; cancel.
     rewrite LOG.intact_idempred; cancel.
     rewrite LOG.notxn_idempred; cancel.
- Qed.
-
+  Qed.
 
   Theorem file_getattr_recover_ok : forall fsxp inum mscs,
   {<< ds pathname Fm Ftop tree f,
@@ -373,7 +345,7 @@ Module AFS.
     subst; pimpl_crash; cancel.
     apply LOG.notxn_intact.
     apply LOG.notxn_intact.
- Qed.
+  Qed.
 
 
   Theorem file_getattr_recover_ok_strict : forall fsxp inum mscs,
@@ -430,8 +402,6 @@ Module AFS.
     cancel; cancel.
   Qed.
 
-
-
   Theorem read_fblock_ok : forall fsxp inum off mscs,
     {< ds Fm Ftop tree pathname f Fd vs,
     PRE    LOG.rep (FSXPLog fsxp) (SB.rep fsxp) (LOG.NoTxn ds) mscs *
@@ -444,16 +414,16 @@ Module AFS.
     CRASH  LOG.intact (FSXPLog fsxp) (SB.rep fsxp) ds
     >} read_fblock fsxp inum off mscs.
   Proof.
-      unfold read_fblock; intros.
-      step.
-      step.
-      eapply pimpl_ok2.
-      apply LOG.commit_ro_ok.
-      cancel.
-      step.
-      subst; pimpl_crash; cancel.
-      apply LOG.notxn_intact.
-      apply LOG.notxn_intact.
+    unfold read_fblock; intros.
+    step.
+    step.
+    eapply pimpl_ok2.
+    apply LOG.commit_ro_ok.
+    cancel.
+    step.
+    subst; pimpl_crash; cancel.
+    apply LOG.notxn_intact.
+    apply LOG.notxn_intact.
   Qed.
 
 
@@ -513,9 +483,78 @@ Module AFS.
 
     step.
     cancel; cancel.
-
   Qed.
 
+  Theorem file_truncate_ok : forall fsxp inum sz mscs,
+    {< ds Fm flist A f,
+    PRE
+      LOG.rep (FSXPLog fsxp) (SB.rep fsxp) (LOG.NoTxn ds) mscs *
+      [[[ ds!! ::: (Fm * BFILE.rep (FSXPBlockAlloc fsxp) (FSXPInode fsxp) flist) ]]] *
+      [[[ flist ::: (A * inum |-> f) ]]]
+    POST RET:^(mscs, r)
+      [[ r = false ]] * LOG.rep (FSXPLog fsxp) (SB.rep fsxp) (LOG.NoTxn ds) mscs \/
+      [[ r = true  ]] * exists d flist' f',
+        LOG.rep (FSXPLog fsxp) (SB.rep fsxp) (LOG.NoTxn (pushd d ds)) mscs *
+        [[[ d :::(Fm * BFILE.rep (FSXPBlockAlloc fsxp) (FSXPInode fsxp) flist') ]]] *
+        [[[ flist' ::: (A * inum |-> f') ]]] *
+        [[ f' = BFILE.mk_bfile (setlen (BFILE.BFData f) sz ($0, nil)) (BFILE.BFAttr f) ]]
+    CRASH
+      LOG.intact (FSXPLog fsxp) (SB.rep fsxp) ds
+     >} file_truncate fsxp inum sz mscs.
+  Proof.
+    unfold file_truncate; intros.
+    step.
+    step.
+    destruct a0.
+    step.
+    step.
+    step.  (* commit *)
+    step.
+    apply LOG.notxn_intact.
+    step.
+    step.  (* abort *)
+    step.
+    apply LOG.notxn_intact.
+    step.
+    apply LOG.notxn_intact.
+  Qed.
+
+  Hint Extern 1 ({{_}} progseq (file_truncate _ _ _ _) _) => apply file_truncate_ok : prog.
+
+  Theorem c_reover_ok : forall fsxp inum sz mscs,
+    {<< ds Fm flist A f,
+    PRE
+      LOG.rep (FSXPLog fsxp) (SB.rep fsxp) (LOG.NoTxn ds) mscs *
+      [[[ ds!! ::: (Fm * BFILE.rep (FSXPBlockAlloc fsxp) (FSXPInode fsxp) flist) ]]] *
+      [[[ flist ::: (A * inum |-> f) ]]]
+    POST RET:^(mscs, r)
+      [[ r = false ]] * LOG.rep (FSXPLog fsxp) (SB.rep fsxp) (LOG.NoTxn ds) mscs \/
+      [[ r = true  ]] * exists d flist' f',
+        LOG.rep (FSXPLog fsxp) (SB.rep fsxp) (LOG.NoTxn (pushd d ds)) mscs *
+        [[[ d :::(Fm * BFILE.rep (FSXPBlockAlloc fsxp) (FSXPInode fsxp) flist') ]]] *
+        [[[ flist' ::: (A * inum |-> f') ]]] *
+        [[ f' = BFILE.mk_bfile (setlen (BFILE.BFData f) sz ($0, nil)) (BFILE.BFAttr f) ]]
+    REC RET:^(mscs,fsxp)
+      exists d, LOG.rep (FSXPLog fsxp) (SB.rep fsxp) (LOG.NoTxn (d, nil)) mscs *
+         [[[ d ::: crash_xform (diskIs (list2nmem (fst ds))) ]]]
+     >>} file_truncate fsxp inum sz mscs >> recover.
+  Proof.
+    unfold forall_helper.
+    intros; eexists; intros.
+    eapply pimpl_ok3.
+    eapply corr3_from_corr2_rx.
+    eapply file_truncate_ok.
+    eapply recover_ok.
+    cancel.
+    step.
+    eassign ( LOG.intact (FSXPLog fsxp) (SB.rep fsxp) v \/
+      (exists cs : cachestate, LOG.after_crash (FSXPLog fsxp) (SB.rep fsxp) (fst v, []) cs))%pred.
+    xform_norm.
+    recover_ro_ok.
+    cancel.
+    or_l.
+    (* rewrite LOG.crash_xform_intact. *)
+  Admitted.
 
   Theorem update_fblock_d_ok : forall fsxp inum off v mscs,
     {< ds Fm flist A f Fd v0,
@@ -620,178 +659,178 @@ Module AFS.
   Qed.
 
 (*
-Theorem create_ok : forall fsxp dnum name mscs,
-  {< m pathname Fm Ftop tree tree_elem,
-  PRE     LOG.rep (FSXPLog fsxp) (sb_rep fsxp) (NoTransaction m) mscs *
-          [[ (Fm * DIRTREE.rep fsxp Ftop tree)%pred (list2mem m) ]] *
-          [[ DIRTREE.find_subtree pathname tree = Some (DIRTREE.TreeDir dnum tree_elem) ]]
-  POST RET:^(mscs,r)
-          [[ r = None ]] * LOG.rep (FSXPLog fsxp) (sb_rep fsxp) (NoTransaction m) mscs \/
-           (exists m', LOG.rep (FSXPLog fsxp) (sb_rep fsxp) (NoTransaction m') mscs *
-            exists inum tree', [[ r = Some inum ]] *
-            [[ tree' = DIRTREE.tree_graft dnum tree_elem pathname name 
-                         (DIRTREE.TreeFile inum BFILE.bfile0) tree ]] *
-            [[ (Fm * DIRTREE.rep fsxp Ftop tree')%pred (list2mem m') ]])
-  CRASH   LOG.would_recover_either_pred (FSXPLog fsxp) (sb_rep fsxp) m (
-            exists inum tree',
-            (Fm * DIRTREE.rep fsxp Ftop tree') *
-            [[ tree' = DIRTREE.tree_graft dnum tree_elem pathname name 
-                         (DIRTREE.TreeFile inum BFILE.bfile0) tree ]])
-  >} create fsxp dnum name mscs.
-Proof.
-  unfold create.
-  hoare.
-  erewrite DIRTREE.find_subtree_tree_graft by eauto; reflexivity.
-  eapply pimpl_or_r; right; cancel.
-  erewrite DIRTREE.update_subtree_tree_graft by eauto; reflexivity.
-  all: try rewrite LOG.activetxn_would_recover_old.
-  all: try rewrite LOG.notxn_would_recover_old.
-  all: try apply LOG.would_recover_old_either_pred.
-  rewrite <- LOG.would_recover_either_pred_pimpl.
-  cancel.
-  erewrite DIRTREE.update_subtree_tree_graft by eauto; reflexivity.
-  Grab Existential Variables.
-  all: eauto.
-  exact BFILE.bfile0.
-Qed.
+  Theorem create_ok : forall fsxp dnum name mscs,
+    {< m pathname Fm Ftop tree tree_elem,
+    PRE     LOG.rep (FSXPLog fsxp) (sb_rep fsxp) (NoTransaction m) mscs *
+            [[ (Fm * DIRTREE.rep fsxp Ftop tree)%pred (list2mem m) ]] *
+            [[ DIRTREE.find_subtree pathname tree = Some (DIRTREE.TreeDir dnum tree_elem) ]]
+    POST RET:^(mscs,r)
+            [[ r = None ]] * LOG.rep (FSXPLog fsxp) (sb_rep fsxp) (NoTransaction m) mscs \/
+             (exists m', LOG.rep (FSXPLog fsxp) (sb_rep fsxp) (NoTransaction m') mscs *
+              exists inum tree', [[ r = Some inum ]] *
+              [[ tree' = DIRTREE.tree_graft dnum tree_elem pathname name 
+                           (DIRTREE.TreeFile inum BFILE.bfile0) tree ]] *
+              [[ (Fm * DIRTREE.rep fsxp Ftop tree')%pred (list2mem m') ]])
+    CRASH   LOG.would_recover_either_pred (FSXPLog fsxp) (sb_rep fsxp) m (
+              exists inum tree',
+              (Fm * DIRTREE.rep fsxp Ftop tree') *
+              [[ tree' = DIRTREE.tree_graft dnum tree_elem pathname name 
+                           (DIRTREE.TreeFile inum BFILE.bfile0) tree ]])
+    >} create fsxp dnum name mscs.
+  Proof.
+    unfold create.
+    hoare.
+    erewrite DIRTREE.find_subtree_tree_graft by eauto; reflexivity.
+    eapply pimpl_or_r; right; cancel.
+    erewrite DIRTREE.update_subtree_tree_graft by eauto; reflexivity.
+    all: try rewrite LOG.activetxn_would_recover_old.
+    all: try rewrite LOG.notxn_would_recover_old.
+    all: try apply LOG.would_recover_old_either_pred.
+    rewrite <- LOG.would_recover_either_pred_pimpl.
+    cancel.
+    erewrite DIRTREE.update_subtree_tree_graft by eauto; reflexivity.
+    Grab Existential Variables.
+    all: eauto.
+    exact BFILE.bfile0.
+  Qed.
 
-Hint Extern 1 ({{_}} progseq (create _ _ _ _ ) _) => apply create_ok : prog.
+  Hint Extern 1 ({{_}} progseq (create _ _ _ _ ) _) => apply create_ok : prog.
 
-Theorem create_recover_ok : forall fsxp dnum name mscs,
-  {<< m pathname Fm Ftop tree tree_elem,
-  PRE     [[ cachesize <> 0 ]] *
-          LOG.rep (FSXPLog fsxp) (sb_rep fsxp) (NoTransaction m) mscs *
-          [[ (Fm * DIRTREE.rep fsxp Ftop tree)%pred (list2mem m) ]] *
-          [[ DIRTREE.find_subtree pathname tree = Some (DIRTREE.TreeDir dnum tree_elem) ]]
-  POST RET:^(mscs,r)
-          [[ r = None ]] * LOG.rep (FSXPLog fsxp) (sb_rep fsxp) (NoTransaction m) mscs \/
-          (exists m', LOG.rep (FSXPLog fsxp) (sb_rep fsxp) (NoTransaction m') mscs *
-            exists inum tree', [[ r = Some inum ]] *
-            [[ tree' = DIRTREE.tree_graft dnum tree_elem pathname name 
-                         (DIRTREE.TreeFile inum BFILE.bfile0) tree  ]] *
-            [[ (Fm * DIRTREE.rep fsxp Ftop tree')%pred (list2mem m') ]])
-  REC RET:^(mscs,fsxp)
-          LOG.rep (FSXPLog fsxp) (sb_rep fsxp) (NoTransaction m) mscs \/ exists m',
-          LOG.rep (FSXPLog fsxp) (sb_rep fsxp) (NoTransaction m') mscs *
-           exists inum tree',
-            [[ tree' = DIRTREE.tree_graft dnum tree_elem pathname name 
-                         (DIRTREE.TreeFile inum BFILE.bfile0) tree  ]] *
-            [[ (Fm * DIRTREE.rep fsxp Ftop tree')%pred (list2mem m') ]]
-  >>} create fsxp dnum name mscs >> recover.
-Proof.
-  recover_rw_ok.
-Qed.
+  Theorem create_recover_ok : forall fsxp dnum name mscs,
+    {<< m pathname Fm Ftop tree tree_elem,
+    PRE     [[ cachesize <> 0 ]] *
+            LOG.rep (FSXPLog fsxp) (sb_rep fsxp) (NoTransaction m) mscs *
+            [[ (Fm * DIRTREE.rep fsxp Ftop tree)%pred (list2mem m) ]] *
+            [[ DIRTREE.find_subtree pathname tree = Some (DIRTREE.TreeDir dnum tree_elem) ]]
+    POST RET:^(mscs,r)
+            [[ r = None ]] * LOG.rep (FSXPLog fsxp) (sb_rep fsxp) (NoTransaction m) mscs \/
+            (exists m', LOG.rep (FSXPLog fsxp) (sb_rep fsxp) (NoTransaction m') mscs *
+              exists inum tree', [[ r = Some inum ]] *
+              [[ tree' = DIRTREE.tree_graft dnum tree_elem pathname name 
+                           (DIRTREE.TreeFile inum BFILE.bfile0) tree  ]] *
+              [[ (Fm * DIRTREE.rep fsxp Ftop tree')%pred (list2mem m') ]])
+    REC RET:^(mscs,fsxp)
+            LOG.rep (FSXPLog fsxp) (sb_rep fsxp) (NoTransaction m) mscs \/ exists m',
+            LOG.rep (FSXPLog fsxp) (sb_rep fsxp) (NoTransaction m') mscs *
+             exists inum tree',
+              [[ tree' = DIRTREE.tree_graft dnum tree_elem pathname name 
+                           (DIRTREE.TreeFile inum BFILE.bfile0) tree  ]] *
+              [[ (Fm * DIRTREE.rep fsxp Ftop tree')%pred (list2mem m') ]]
+    >>} create fsxp dnum name mscs >> recover.
+  Proof.
+    recover_rw_ok.
+  Qed.
 
-Theorem lookup_ok: forall fsxp dnum fnlist mscs,
-  {< m Fm Ftop tree,
-  PRE     LOG.rep (FSXPLog fsxp) (sb_rep fsxp) (NoTransaction m) mscs *
-           [[ (Fm * DIRTREE.rep fsxp Ftop tree)%pred (list2mem m) ]] *
-           [[ dnum = DIRTREE.dirtree_inum tree ]] *
-           [[ DIRTREE.dirtree_isdir tree = true ]]
-  POST RET:^(mscs,r)
-           LOG.rep (FSXPLog fsxp) (sb_rep fsxp) (NoTransaction m) mscs *
-           [[ r = DIRTREE.find_name fnlist tree ]]
-  CRASH   LOG.would_recover_either (FSXPLog fsxp) (sb_rep fsxp) m m
-  >} lookup fsxp dnum fnlist mscs.
-Proof.
-  unfold lookup.
-  hoare.
-  apply LOG.would_recover_old_either.
-  rewrite LOG.notxn_would_recover_old. apply LOG.would_recover_old_either.
-  rewrite LOG.activetxn_would_recover_old. apply LOG.would_recover_old_either.
-Qed.
+  Theorem lookup_ok: forall fsxp dnum fnlist mscs,
+    {< m Fm Ftop tree,
+    PRE     LOG.rep (FSXPLog fsxp) (sb_rep fsxp) (NoTransaction m) mscs *
+             [[ (Fm * DIRTREE.rep fsxp Ftop tree)%pred (list2mem m) ]] *
+             [[ dnum = DIRTREE.dirtree_inum tree ]] *
+             [[ DIRTREE.dirtree_isdir tree = true ]]
+    POST RET:^(mscs,r)
+             LOG.rep (FSXPLog fsxp) (sb_rep fsxp) (NoTransaction m) mscs *
+             [[ r = DIRTREE.find_name fnlist tree ]]
+    CRASH   LOG.would_recover_either (FSXPLog fsxp) (sb_rep fsxp) m m
+    >} lookup fsxp dnum fnlist mscs.
+  Proof.
+    unfold lookup.
+    hoare.
+    apply LOG.would_recover_old_either.
+    rewrite LOG.notxn_would_recover_old. apply LOG.would_recover_old_either.
+    rewrite LOG.activetxn_would_recover_old. apply LOG.would_recover_old_either.
+  Qed.
 
-Hint Extern 1 ({{_}} progseq (lookup _ _ _ _) _) => apply lookup_ok : prog.
+  Hint Extern 1 ({{_}} progseq (lookup _ _ _ _) _) => apply lookup_ok : prog.
 
 
-Theorem lookup_recover_ok : forall fsxp dnum fnlist mscs,
-  {<< m Fm Ftop tree,
-  PRE     LOG.rep (FSXPLog fsxp) (sb_rep fsxp) (NoTransaction m) mscs *
-           [[ (Fm * DIRTREE.rep fsxp Ftop tree)%pred (list2mem m) ]] *
-           [[ dnum = DIRTREE.dirtree_inum tree ]] *
-           [[ DIRTREE.dirtree_isdir tree = true ]]
-  POST RET:^(mscs,r)
-           LOG.rep (FSXPLog fsxp) (sb_rep fsxp) (NoTransaction m) mscs *
-           [[ r = DIRTREE.find_name fnlist tree ]]
-  REC RET:^(mscs, fsxp)
-           LOG.rep (FSXPLog fsxp) (sb_rep fsxp) (NoTransaction m) mscs
-  >>} lookup fsxp dnum fnlist mscs >> recover.
-Proof.
-  recover_ro_ok.
-Qed.
+  Theorem lookup_recover_ok : forall fsxp dnum fnlist mscs,
+    {<< m Fm Ftop tree,
+    PRE     LOG.rep (FSXPLog fsxp) (sb_rep fsxp) (NoTransaction m) mscs *
+             [[ (Fm * DIRTREE.rep fsxp Ftop tree)%pred (list2mem m) ]] *
+             [[ dnum = DIRTREE.dirtree_inum tree ]] *
+             [[ DIRTREE.dirtree_isdir tree = true ]]
+    POST RET:^(mscs,r)
+             LOG.rep (FSXPLog fsxp) (sb_rep fsxp) (NoTransaction m) mscs *
+             [[ r = DIRTREE.find_name fnlist tree ]]
+    REC RET:^(mscs, fsxp)
+             LOG.rep (FSXPLog fsxp) (sb_rep fsxp) (NoTransaction m) mscs
+    >>} lookup fsxp dnum fnlist mscs >> recover.
+  Proof.
+    recover_ro_ok.
+  Qed.
 
-Theorem rename_ok : forall fsxp dnum srcpath srcname dstpath dstname mscs,
-  {< m Ftop tree cwd tree_elem,
-  PRE     LOG.rep (FSXPLog fsxp) (sb_rep fsxp) (NoTransaction m) mscs *
-          [[ (DIRTREE.rep fsxp Ftop tree) (list2mem m) ]] *
-          [[ DIRTREE.find_subtree cwd tree = Some (DIRTREE.TreeDir dnum tree_elem) ]]
-  POST RET:^(mscs,ok)
-          [[ ok = false ]] * LOG.rep (FSXPLog fsxp) (sb_rep fsxp) (NoTransaction m) mscs \/
-          [[ ok = true ]] * exists m' srcnum srcents dstnum dstents subtree pruned renamed tree',
-          LOG.rep (FSXPLog fsxp) (sb_rep fsxp) (NoTransaction m') mscs *
-          [[ (DIRTREE.rep fsxp Ftop tree')%pred (list2mem m') ]] *
-          [[ DIRTREE.find_subtree srcpath (DIRTREE.TreeDir dnum tree_elem) = Some (DIRTREE.TreeDir srcnum srcents) ]] *
-          [[ DIRTREE.find_dirlist srcname srcents = Some subtree ]] *
-          [[ pruned = DIRTREE.tree_prune srcnum srcents srcpath srcname (DIRTREE.TreeDir dnum tree_elem) ]] *
-          [[ DIRTREE.find_subtree dstpath pruned = Some (DIRTREE.TreeDir dstnum dstents) ]] *
-          [[ renamed = DIRTREE.tree_graft dstnum dstents dstpath dstname subtree pruned ]] *
-          [[ tree' = DIRTREE.update_subtree cwd renamed tree ]]
-  CRASH   LOG.would_recover_either_pred (FSXPLog fsxp) (sb_rep fsxp) m (
-          exists srcnum srcents dstnum dstents subtree pruned renamed tree',
-          (DIRTREE.rep fsxp Ftop tree')%pred *
-          [[ DIRTREE.find_subtree srcpath (DIRTREE.TreeDir dnum tree_elem) = Some (DIRTREE.TreeDir srcnum srcents) ]] *
-          [[ DIRTREE.find_dirlist srcname srcents = Some subtree ]] *
-          [[ pruned = DIRTREE.tree_prune srcnum srcents srcpath srcname (DIRTREE.TreeDir dnum tree_elem) ]] *
-          [[ DIRTREE.find_subtree dstpath pruned = Some (DIRTREE.TreeDir dstnum dstents) ]] *
-          [[ renamed = DIRTREE.tree_graft dstnum dstents dstpath dstname subtree pruned ]] *
-          [[ tree' = DIRTREE.update_subtree cwd renamed tree ]])
-  >} rename fsxp dnum srcpath srcname dstpath dstname mscs.
-Proof.
-  unfold rename.
-  hoare.
-  all: try rewrite LOG.activetxn_would_recover_old.
-  all: try rewrite LOG.notxn_would_recover_old.
-  all: try apply LOG.would_recover_old_either_pred.
-  rewrite <- LOG.would_recover_either_pred_pimpl.
-  cancel.
-Qed.
+  Theorem rename_ok : forall fsxp dnum srcpath srcname dstpath dstname mscs,
+    {< m Ftop tree cwd tree_elem,
+    PRE     LOG.rep (FSXPLog fsxp) (sb_rep fsxp) (NoTransaction m) mscs *
+            [[ (DIRTREE.rep fsxp Ftop tree) (list2mem m) ]] *
+            [[ DIRTREE.find_subtree cwd tree = Some (DIRTREE.TreeDir dnum tree_elem) ]]
+    POST RET:^(mscs,ok)
+            [[ ok = false ]] * LOG.rep (FSXPLog fsxp) (sb_rep fsxp) (NoTransaction m) mscs \/
+            [[ ok = true ]] * exists m' srcnum srcents dstnum dstents subtree pruned renamed tree',
+            LOG.rep (FSXPLog fsxp) (sb_rep fsxp) (NoTransaction m') mscs *
+            [[ (DIRTREE.rep fsxp Ftop tree')%pred (list2mem m') ]] *
+            [[ DIRTREE.find_subtree srcpath (DIRTREE.TreeDir dnum tree_elem) = Some (DIRTREE.TreeDir srcnum srcents) ]] *
+            [[ DIRTREE.find_dirlist srcname srcents = Some subtree ]] *
+            [[ pruned = DIRTREE.tree_prune srcnum srcents srcpath srcname (DIRTREE.TreeDir dnum tree_elem) ]] *
+            [[ DIRTREE.find_subtree dstpath pruned = Some (DIRTREE.TreeDir dstnum dstents) ]] *
+            [[ renamed = DIRTREE.tree_graft dstnum dstents dstpath dstname subtree pruned ]] *
+            [[ tree' = DIRTREE.update_subtree cwd renamed tree ]]
+    CRASH   LOG.would_recover_either_pred (FSXPLog fsxp) (sb_rep fsxp) m (
+            exists srcnum srcents dstnum dstents subtree pruned renamed tree',
+            (DIRTREE.rep fsxp Ftop tree')%pred *
+            [[ DIRTREE.find_subtree srcpath (DIRTREE.TreeDir dnum tree_elem) = Some (DIRTREE.TreeDir srcnum srcents) ]] *
+            [[ DIRTREE.find_dirlist srcname srcents = Some subtree ]] *
+            [[ pruned = DIRTREE.tree_prune srcnum srcents srcpath srcname (DIRTREE.TreeDir dnum tree_elem) ]] *
+            [[ DIRTREE.find_subtree dstpath pruned = Some (DIRTREE.TreeDir dstnum dstents) ]] *
+            [[ renamed = DIRTREE.tree_graft dstnum dstents dstpath dstname subtree pruned ]] *
+            [[ tree' = DIRTREE.update_subtree cwd renamed tree ]])
+    >} rename fsxp dnum srcpath srcname dstpath dstname mscs.
+  Proof.
+    unfold rename.
+    hoare.
+    all: try rewrite LOG.activetxn_would_recover_old.
+    all: try rewrite LOG.notxn_would_recover_old.
+    all: try apply LOG.would_recover_old_either_pred.
+    rewrite <- LOG.would_recover_either_pred_pimpl.
+    cancel.
+  Qed.
 
-Hint Extern 1 ({{_}} progseq (rename _ _ _ _ _ _ _) _) => apply rename_ok : prog.
+  Hint Extern 1 ({{_}} progseq (rename _ _ _ _ _ _ _) _) => apply rename_ok : prog.
 
-(* XXX Use rep_return spec in App.v? *)
-Theorem rename_recover_ok : forall fsxp dnum srcpath srcname dstpath dstname mscs,
-  {<< m Ftop tree cwd tree_elem,
-  PRE     LOG.rep (FSXPLog fsxp) (sb_rep fsxp) (NoTransaction m) mscs *
-          [[ (DIRTREE.rep fsxp Ftop tree) (list2mem m) ]] *
-          [[ DIRTREE.find_subtree cwd tree = Some (DIRTREE.TreeDir dnum tree_elem) ]]
-  POST RET:^(mscs,ok)
-          [[ ok = false ]] * LOG.rep (FSXPLog fsxp) (sb_rep fsxp) (NoTransaction m) mscs \/
-          [[ ok = true ]] * exists m' srcnum srcents dstnum dstents subtree pruned renamed tree',
-          LOG.rep (FSXPLog fsxp) (sb_rep fsxp) (NoTransaction m') mscs *
-          [[ (DIRTREE.rep fsxp Ftop tree')%pred (list2mem m') ]] *
-          [[ DIRTREE.find_subtree srcpath (DIRTREE.TreeDir dnum tree_elem) = Some (DIRTREE.TreeDir srcnum srcents) ]] *
-          [[ DIRTREE.find_dirlist srcname srcents = Some subtree ]] *
-          [[ pruned = DIRTREE.tree_prune srcnum srcents srcpath srcname (DIRTREE.TreeDir dnum tree_elem) ]] *
-          [[ DIRTREE.find_subtree dstpath pruned = Some (DIRTREE.TreeDir dstnum dstents) ]] *
-          [[ renamed = DIRTREE.tree_graft dstnum dstents dstpath dstname subtree pruned ]] *
-          [[ tree' = DIRTREE.update_subtree cwd renamed tree ]]
-  REC RET:^(mscs,fsxp)
-          LOG.rep (FSXPLog fsxp) (sb_rep fsxp) (NoTransaction m) mscs \/
-          exists m' srcnum srcents dstnum dstents subtree pruned renamed tree',
-          LOG.rep (FSXPLog fsxp) (sb_rep fsxp) (NoTransaction m') mscs *
-          [[ (DIRTREE.rep fsxp Ftop tree')%pred (list2mem m') ]] *
-          [[ DIRTREE.find_subtree srcpath (DIRTREE.TreeDir dnum tree_elem) = Some (DIRTREE.TreeDir srcnum srcents) ]] *
-          [[ DIRTREE.find_dirlist srcname srcents = Some subtree ]] *
-          [[ pruned = DIRTREE.tree_prune srcnum srcents srcpath srcname (DIRTREE.TreeDir dnum tree_elem) ]] *
-          [[ DIRTREE.find_subtree dstpath pruned = Some (DIRTREE.TreeDir dstnum dstents) ]] *
-          [[ renamed = DIRTREE.tree_graft dstnum dstents dstpath dstname subtree pruned ]] *
-          [[ tree' = DIRTREE.update_subtree cwd renamed tree ]]
-  >>} rename fsxp dnum srcpath srcname dstpath dstname mscs >> recover.
-Proof.
-  recover_rw_ok.
-Qed.
+  (* XXX Use rep_return spec in App.v? *)
+  Theorem rename_recover_ok : forall fsxp dnum srcpath srcname dstpath dstname mscs,
+    {<< m Ftop tree cwd tree_elem,
+    PRE     LOG.rep (FSXPLog fsxp) (sb_rep fsxp) (NoTransaction m) mscs *
+            [[ (DIRTREE.rep fsxp Ftop tree) (list2mem m) ]] *
+            [[ DIRTREE.find_subtree cwd tree = Some (DIRTREE.TreeDir dnum tree_elem) ]]
+    POST RET:^(mscs,ok)
+            [[ ok = false ]] * LOG.rep (FSXPLog fsxp) (sb_rep fsxp) (NoTransaction m) mscs \/
+            [[ ok = true ]] * exists m' srcnum srcents dstnum dstents subtree pruned renamed tree',
+            LOG.rep (FSXPLog fsxp) (sb_rep fsxp) (NoTransaction m') mscs *
+            [[ (DIRTREE.rep fsxp Ftop tree')%pred (list2mem m') ]] *
+            [[ DIRTREE.find_subtree srcpath (DIRTREE.TreeDir dnum tree_elem) = Some (DIRTREE.TreeDir srcnum srcents) ]] *
+            [[ DIRTREE.find_dirlist srcname srcents = Some subtree ]] *
+            [[ pruned = DIRTREE.tree_prune srcnum srcents srcpath srcname (DIRTREE.TreeDir dnum tree_elem) ]] *
+            [[ DIRTREE.find_subtree dstpath pruned = Some (DIRTREE.TreeDir dstnum dstents) ]] *
+            [[ renamed = DIRTREE.tree_graft dstnum dstents dstpath dstname subtree pruned ]] *
+            [[ tree' = DIRTREE.update_subtree cwd renamed tree ]]
+    REC RET:^(mscs,fsxp)
+            LOG.rep (FSXPLog fsxp) (sb_rep fsxp) (NoTransaction m) mscs \/
+            exists m' srcnum srcents dstnum dstents subtree pruned renamed tree',
+            LOG.rep (FSXPLog fsxp) (sb_rep fsxp) (NoTransaction m') mscs *
+            [[ (DIRTREE.rep fsxp Ftop tree')%pred (list2mem m') ]] *
+            [[ DIRTREE.find_subtree srcpath (DIRTREE.TreeDir dnum tree_elem) = Some (DIRTREE.TreeDir srcnum srcents) ]] *
+            [[ DIRTREE.find_dirlist srcname srcents = Some subtree ]] *
+            [[ pruned = DIRTREE.tree_prune srcnum srcents srcpath srcname (DIRTREE.TreeDir dnum tree_elem) ]] *
+            [[ DIRTREE.find_subtree dstpath pruned = Some (DIRTREE.TreeDir dstnum dstents) ]] *
+            [[ renamed = DIRTREE.tree_graft dstnum dstents dstpath dstname subtree pruned ]] *
+            [[ tree' = DIRTREE.update_subtree cwd renamed tree ]]
+    >>} rename fsxp dnum srcpath srcname dstpath dstname mscs >> recover.
+  Proof.
+    recover_rw_ok.
+  Qed.
 
-*)
+  *)
 
 End AFS.
 
